cleanup

src/boss/bossLib.sig
@@ -213,7 +213,7 @@ sig
   val name_ind_cases : term list -> thm -> thm
 
   (* convert aux size operators to combinators and use append rules *)
-  val size_comb_tac : tactic
+(*  val size_comb_tac : tactic *)
 
   (* more simplification variants *)
   val fsrw_tac : simpLib.ssfrag list -> thm list -> tactic
