src/Boolify/src/EncodeScript.sml
@@ -1,8 +1,3 @@
-(* Interactive mode
-app load
-["bossLib", "listSyntax", "combinSyntax", "rich_listTheory", "metisLib"];
-*)
-
 open HolKernel boolLib Parse bossLib pairTheory pairTools combinTheory
      arithmeticTheory listTheory rich_listTheory optionTheory metisLib;
 
@@ -21,7 +16,9 @@ val TOP_CASE_TAC = BasicProvers.TOP_CASE_TAC;
         biprefix is a bi-directional version of IS_PREFIX.
  ---------------------------------------------------------------------------*)
 
-val biprefix_def = Define `biprefix a b <=> IS_PREFIX a b \/ IS_PREFIX b a`;
+Definition biprefix_def:
+ biprefix a b <=> IS_PREFIX a b \/ IS_PREFIX b a
+End
 
 val biprefix_refl = store_thm
   ("biprefix_refl",
@@ -103,7 +100,9 @@ val lift_tree_total = store_thm
         Well-formed predicates are non-empty.
  ---------------------------------------------------------------------------*)
 
-val wf_pred_def = Define `wf_pred p = ?x. p x`;
+Definition wf_pred_def:
+ wf_pred p = ?x. p x
+End
 
 (*---------------------------------------------------------------------------
         A well-formed encoder is prefix-free and injective.
@@ -134,8 +133,9 @@ val wf_encoder_total = store_thm
       target list: the type has all the information!
  ---------------------------------------------------------------------------*)
 
-val encode_unit_def =
-  TotalDefn.Define `encode_unit (_ : one) : bool list = []`;
+Definition encode_unit_def:
+  encode_unit (_ : one) : bool list = []
+End
 
 val wf_encode_unit = store_thm
   ("wf_encode_unit",
@@ -146,8 +146,9 @@ val wf_encode_unit = store_thm
         Booleans
  ---------------------------------------------------------------------------*)
 
-val encode_bool_def = TotalDefn.Define
-  `encode_bool (x : bool) = [x]`;
+Definition encode_bool_def:
+  encode_bool (x : bool) = [x]
+End
 
 val wf_encode_bool = store_thm
   ("wf_encode_bool",
@@ -158,11 +159,13 @@ val wf_encode_bool = store_thm
         Pairs
  ---------------------------------------------------------------------------*)
 
-val encode_prod_def =
-  TotalDefn.Define
-  `encode_prod xb yb (x : 'a, y : 'b) : bool list = APPEND (xb x) (yb y)`;
+Definition encode_prod_def:
+  encode_prod xb yb (x : 'a, y : 'b) : bool list = APPEND (xb x) (yb y)
+End
 
-val lift_prod_def = Define `lift_prod p1 p2 x <=> p1 (FST x) /\ p2 (SND x)`;
+Definition lift_prod_def:
+  lift_prod p1 p2 x <=> p1 (FST x) /\ p2 (SND x)
+End
 
 val encode_prod_alt = store_thm
   ("encode_prod_alt",
@@ -186,14 +189,15 @@ val wf_encode_prod = store_thm
         Sums
  ---------------------------------------------------------------------------*)
 
-val encode_sum_def =
-  TotalDefn.Define
-  `(encode_sum xb yb (INL (x : 'a)) : bool list = T :: xb x) /\
-   (encode_sum xb yb (INR (y : 'b)) = F :: yb y)`;
+Definition encode_sum_def:
+  (encode_sum xb yb (INL (x : 'a)) : bool list = T :: xb x) /\
+  (encode_sum xb yb (INR (y : 'b)) = F :: yb y)
+End
 
-val lift_sum_def = Define
-  `lift_sum (p1 : 'a->bool) p2 x =
-   case x of INL x1 => p1 x1 | INR x2 => p2 x2`;
+Definition lift_sum_def:
+  lift_sum (p1 : 'a->bool) p2 x =
+   case x of INL x1 => p1 x1 | INR x2 => p2 x2
+End
 
 val wf_encode_sum = store_thm
   ("wf_encode_sum",
@@ -209,13 +213,14 @@ val wf_encode_sum = store_thm
         Options
  ---------------------------------------------------------------------------*)
 
-val encode_option_def =
-  TotalDefn.Define
-  `(encode_option xb NONE = [F]) /\
-   (encode_option xb (SOME x) = T :: xb x)`;
+Definition encode_option_def:
+  encode_option xb NONE = [F] /\
+  encode_option xb (SOME x) = T :: xb x
+End
 
-val lift_option_def = Define
-  `lift_option p x = case x of NONE => T | SOME y => p y`;
+Definition lift_option_def:
+  lift_option p x = case x of NONE => T | SOME y => p y
+End
 
 val wf_encode_option = store_thm
   ("wf_encode_option",
@@ -229,10 +234,10 @@ val wf_encode_option = store_thm
         Lists
  ---------------------------------------------------------------------------*)
 
-val encode_list_def =
-  TotalDefn.Define
-  `(encode_list xb [] = [F]) /\
-   (encode_list xb (x :: xs) = T :: APPEND (xb x) (encode_list xb xs))`;
+Definition encode_list_def:
+  (encode_list xb [] = [F]) /\
+  (encode_list xb (x :: xs) = T :: APPEND (xb x) (encode_list xb xs))
+End
 
 val wf_encode_list = store_thm
   ("wf_encode_list",
@@ -272,12 +277,14 @@ QED
         Bounded lists
  ---------------------------------------------------------------------------*)
 
-val encode_blist_def =
-  Define
-  `(encode_blist 0 e l = []) /\
-   (encode_blist (SUC m) e l = APPEND (e (HD l)) (encode_blist m e (TL l)))`;
+Definition encode_blist_def:
+  (encode_blist 0 e l = []) /\
+  (encode_blist (SUC m) e l = APPEND (e (HD l)) (encode_blist m e (TL l)))
+End
 
-val lift_blist_def = Define `lift_blist m p x <=> EVERY p x /\ (LENGTH x = m)`;
+Definition lift_blist_def:
+  lift_blist m p x <=> EVERY p x /\ (LENGTH x = m)
+End
 
 Theorem lift_blist_suc:
    !n p h t. lift_blist (SUC n) p (h :: t) <=> p h /\ lift_blist n p t
@@ -310,31 +317,16 @@ val wf_encode_blist = store_thm
         Nums (Norrish numeral encoding)
  ---------------------------------------------------------------------------*)
 
-val (encode_num_def, encode_num_ind) =
-  Defn.tprove
-  (Defn.Hol_defn "encode_num"
-   `encode_num (n:num) =
+Definition encode_num_def:
+  encode_num (n:num) =
     if n = 0 then [T; T]
     else if EVEN n then F :: encode_num ((n - 2) DIV 2)
-    else T :: F :: encode_num ((n - 1) DIV 2)`,
-   TotalDefn.WF_REL_TAC `$<` >>
-   REPEAT STRIP_TAC >>
-   (KNOW_TAC (Term `?j. n = SUC j`) >- PROVE_TAC [num_CASES]) >>
-   STRIP_TAC >>
-   IMP_RES_TAC EVEN_EXISTS >>
-   ASM_SIMP_TAC arith_ss
-   [SUC_SUB1, MULT_DIV, DIV_LESS_EQ,
-    DECIDE (Term `2n*m - 2n = (m-1n)*2n`),
-    DECIDE “x < SUC y <=> x <= y”]);
+    else T :: F :: encode_num ((n - 1) DIV 2)
+Termination
+  WF_REL_TAC ‘$<’ >> simp[DIV_LT_X]
+End
 
-val _ = save_thm ("encode_num_def", encode_num_def);
-val _ = save_thm ("encode_num_ind", encode_num_ind);
-
-  (*--------------------------------------------------------------------
-       Termination proof can also go:
-           WF_REL_TAC `$<` THEN intLib.COOPER_TAC
-       but then we'd need integers.
-   ----------------------------------------------------------------------*)
+val encode_num_def = SPEC_ALL encode_num_def
 
 val wf_encode_num = store_thm
   ("wf_encode_num",
@@ -391,18 +383,19 @@ val wf_encode_num = store_thm
         Bounded numbers (bit encoding)
  ---------------------------------------------------------------------------*)
 
-val encode_bnum_def =
-  Define
-  `(encode_bnum 0 (n : num) = []) /\
-   (encode_bnum (SUC m) n = ~(EVEN n) :: encode_bnum m (n DIV 2))`;
+Definition encode_bnum_def:
+  (encode_bnum 0 (n : num) = []) /\
+  (encode_bnum (SUC m) n = ~(EVEN n) :: encode_bnum m (n DIV 2))
+End
 
-val collision_free_def =
-  Define
-  `collision_free m p =
-   !x y. p x /\ p y /\ (x MOD (2 EXP m) = y MOD (2 EXP m)) ==> (x = y)`;
+Definition collision_free_def:
+  collision_free m p =
+   !x y. p x /\ p y /\ (x MOD (2 EXP m) = y MOD (2 EXP m)) ==> (x = y)
+End
 
-val wf_pred_bnum_def =
-  Define `wf_pred_bnum m p <=> wf_pred p /\ !x. p x ==> x < 2 ** m`;
+Definition wf_pred_bnum_def:
+  wf_pred_bnum m p <=> wf_pred p /\ !x. p x ==> x < 2 ** m
+End
 
 val wf_pred_bnum_total = store_thm
   ("wf_pred_bnum_total",
@@ -516,9 +509,25 @@ val wf_encode_bnum = store_thm
         A challenging example for boolification.
  ---------------------------------------------------------------------------*)
 
-val () = Hol_datatype `tree = Node of 'a => tree list`;
+Datatype:
+  tree = Node 'a (tree list)
+End
 
-val tree_size_def  = fetch "-" "tree_size_def";
+Definition encode_tree_def:
+  encode_tree e (Node a ts) = (e a) ++ encode_list (encode_tree e) ts
+End
+
+Definition lift_tree_def:
+  lift_tree p (Node a ts) <=> p a /\ EVERY (lift_tree p) ts
+End
+
+Theorem encode_tree_def[allow_rebind] =
+        CONV_RULE (DEPTH_CONV ETA_CONV) encode_tree_def
+
+Theorem lift_tree_def[allow_rebind] =
+        CONV_RULE (DEPTH_CONV ETA_CONV) lift_tree_def;
+
+
 val tree_induction = fetch "-" "tree_induction";
 
 val tree_ind = store_thm
@@ -531,26 +540,6 @@ val tree_ind = store_thm
    >> RW_TAC std_ss [EVERY_DEF]
    >> Q.PAT_X_ASSUM `!x. Q x` MATCH_MP_TAC
    >> FULL_SIMP_TAC std_ss [EVERY_MEM]);
-
-val (encode_tree_def, _) =
-  Defn.tprove
-  (Defn.Hol_defn "encode_tree"
-   `encode_tree e (Node a ts) = APPEND (e a) (encode_list (encode_tree e) ts)`,
-   TotalDefn.WF_REL_TAC `measure (tree_size (K 0) o SND)` >>
-   rw [] >> size_comb_tac >> simp []);
-
-val encode_tree_def =
-  save_thm ("encode_tree_def", CONV_RULE (DEPTH_CONV ETA_CONV) encode_tree_def);
-
-val (lift_tree_def, _) =
-  Defn.tprove
-  (Defn.Hol_defn "lift_tree"
-   `lift_tree p (Node a ts) <=> p a /\ EVERY (lift_tree p) ts`,
-   TotalDefn.WF_REL_TAC `measure (tree_size (K 0) o SND)` >>
-   rw_tac bool_ss [] >> size_comb_tac >> simp []);
-
-val lift_tree_def =
-  save_thm ("lift_tree_def", CONV_RULE (DEPTH_CONV ETA_CONV) lift_tree_def);
 
 val wf_encode_tree = store_thm
   ("wf_encode_tree",
