src/boss/bossLib.sml
@@ -355,11 +355,13 @@ end
     useful for proving termination in fold and rose-tree settings
    ---------------------------------------------------------------------- *)
 
+(*
 val size_comb_tac =
   full_simp_tac boolSimps.bool_ss [listTheory.MEM_SPLIT]
   THEN CONV_TAC TotalDefn.size_eq_conv
   THEN simp_tac boolSimps.bool_ss
     [listTheory.list_size_append, listTheory.list_size_def]
+*)
 
 val _ = let
   val sref = TotalDefn.termination_solve_simps
